\documentclass{./../../Latex/homework}
\begin{document}
\thispagestyle{plain}
\newcommand{\mytitle}{Homework 9 Solutions}
\myheader{\mytitle}

%%%%%%%%%%%%%% Exercise 11.2
\subsection*{Exercise 11.2}
\begin{enumerate}

% 1
\item  $z=x^{2}+x y+2 y^{2}+3$ \\

$
\begin{aligned}
&\text {\underline{F.0.C:} } \\
&f_{x}=2 x+y=0 \\
&f_{y}=x+4 y=0
\end{aligned} \\
$

To solve the above system, plug in $x=-4 y$ in the first equation.
$$ 2 x+y=-8 y+y=0 $$

\underline{Critical point:} $(0,0)$ \\

$
\begin{aligned}
&\text {\underline{S.0.C:} } \\
&f_{x x}=2>0 \\
&f_{y y}=4>0 \\
&f_{x y}=1 \\
&f_{x x} f_{y y}=8>1=f_{x y}^{2}
\end{aligned} \\
$

$f$ has a local minimum at $(0,0)$. \\

% 2
\item $z=-x^{2}-y^{2}+6 x+2 y$ \\
 
 \underline{F.0.C:} \\
 $
 \begin{aligned}
&f_{x}=-2 x+6=0 \\
&f_{y}=-2 y+2=0
\end{aligned}
$ \\

\underline{Critical point:} $(3,1)$ \\

 \underline{S.0.C:} \\

$
\begin{aligned}
f_{x x} &=-2<0 \\
f_{y y} &=-2<0 \\
f_{x y} &=0 \\
f_{x x} f_{y y} &=4>0=f_{x y}^{2}
\end{aligned}
$ \\

$f$ has a local maximum at $(3,1)$. \\

% 3
\item $z=a x^{2}+b y^{2}+c$

FOC :

$$
\begin{aligned}
&f_{x}=2 a x=0 \\
&f_{y}=2 b y=0
\end{aligned}
$$

Critical point : $(0,0)$ 

SOC :
$$
\begin{aligned}
&f_{x x}=2 a \\
&f_{y y}=2 b \\
&f_{x y}=0 \\
&f_{x x} f_{y y}=4 a b
\end{aligned}
$$
\begin{enumerate}
\item $a>0, b>0$

$f_{x x}>0, f_{y y}>0$

$f_{x x} f_{y y}=4 a b>0=f^{2}_{x y}$

Local minimum. \\

\item $a<0, b<0$

$f_{x x}<0, f_{y y}<0$

$f_{x x} f_{y y}=4 a b>0=f^{2}_{x y}$

Local maximum. \\

\item $\quad a>0, \quad b<0$

$f_{x x}>0, f_{y y}<0$

Neither maximum nor minimum. \\
\end{enumerate}

% 4
\item $z=e^{2 x}-2 x+2 y^{2}+3$

FOC: 
$$
\begin{aligned}
&f_{x}=2 e^{2 x}-2=0 \rightarrow e^{2 x}=1 \rightarrow 2 x=\ln 1=0 \\
&f_{y}=4 y=0
\end{aligned}
$$

Critical point: $(0,0)$

SOC:

$$
\begin{aligned}
&f_{x x}=4 e^{2 x} \rightarrow f_{x x}(0,0)=4 \\
&f_{y y}=4 \\
&f_{x y}=0
\end{aligned}
$$

At $(0,0)$ :

$$
\begin{aligned}
&f_{x x}>0, f_{y y}>0 \\
&f_{x x} f_{y y}=16>0=f_{x y}^{2} \rightarrow \text { local minimum }
\end{aligned}
$$ \\

% 5
\item  $z=(x-2)^{4}+(y-3)^{4}$ \\
\begin{enumerate}

\item First note that $z \geqslant 0$ as square terms are always positive.

Since, $f(2,3)=0, z$ takes minimum value at $x^{*}=2$ \& $y^{*}=3$. \\

\item $f_{x}=4(x-2)^{3} \rightarrow f_{x}(2,3)=0$

$f_{y}=4(y-3)^{3} \rightarrow f_{y}(2,3)=0$

Yes, FOC is satisfied. \\

\item $f_{x x}(2,3)=12(x-2)^{2} \rightarrow f_{x x}(2,3)=0$

$f_{y y}(2,3)=12(y-3)^{2} \rightarrow f_{yy}(2,3)=0$

$f_{x y}=0$

SOC is not satisfied. 


Yes, the second-order necessary condition is satisfied.
\end{enumerate}

\end{enumerate}

\end{document}